@prefix :       <http://belhisfirm.be/resource/> .
@prefix bhf:    <http://belhisfirm.be/ontology#> .
@prefix owl:    <http://www.w3.org/2002/07/owl#> .
@prefix rdf:    <http://www.w3.org/1999/02/22-rdf-syntax-ns#> .
@prefix xsd:    <http://www.w3.org/2001/XMLSchema#> .
@prefix rdfs:   <http://www.w3.org/2000/01/rdf-schema#> .
@prefix foaf:   <http://xmlns.com/foaf/0.1/> .
@prefix org:    <http://www.w3.org/ns/org#> .
@prefix rov:    <http://www.w3.org/ns/regorg#> .
@prefix schema: <http://schema.org/> .
@prefix dct:    <http://purl.org/dc/terms/> .
@prefix vcard:  <http://www.w3.org/2006/vcard/ns#> .

### General Classes
bhf:Class
    rdf:type owl:Class ;
    rdfs:label "Belhisfirm class"@en ;
    rdfs:comment "A generic class for belhisfirm objects that have other objects as properties" .

bhf:PropertyClass
    rdf:type     owl:Class ;
    rdfs:label   "belhisfirm property class"@en ;
    rdfs:comment "Generic property class for objects that are properties of main classes"@en .

bhf:DatedName
    rdf:type        owl:Class ;
    rdfs:subClassOf bhf:PropertyClass ;
    rdfs:label      "Dated Name"@en, "Gedateerde naam"@nl ;
    rdfs:comment    "Name of an object in Belhisfirm, with a start and end date of the name being valid."@en .


### General properties
bhf:startDate
    rdf:type     owl:DatatypeProperty ;
    rdfs:domain  bhf:PropertyClass ;
    rdfs:range   xsd:date ;
    rdfs:label   "start date"@en, "start datum"@nl ;
    rdfs:comment "Start date of when a property became valid."@en .

bhf:endDate
    rdf:type     owl:DatatypeProperty ;
    rdfs:domain  bhf:PropertyClass ;
    rdfs:range   xsd:date ;
    rdfs:label   "end date"@en, "einde datum"@nl ;
    rdfs:comment "end date of when a property became valid."@en .

bhf:source
    rdf:type     owl:DatatypeProperty ;
    rdfs:domain  bhf:PropertyClass ;
    rdfs:range   xsd:string ;
    rdfs:label   "Source"@en, "Bron"@nl ;
    rdfs:comment "Source of the property"@en .

bhf:comments
    rdf:type     owl:DatatypeProperty ;
    rdfs:domain  bhf:PropertyClass ;
    rdfs:range   xsd:string ;
    rdfs:label   "Comments"@en, "Extra info"@nl ;
    rdfs:comment "Extra info on the property"@en .

bhf:hasName
    rdf:type     owl:ObjectProperty ;
    rdfs:domain  bhf:Class ;
    rdfs:range   bhf:DatedName ;
    rdfs:label   "has dated name"@en, "heeft gedateerde naam"@nl ;
    rdfs:comment "has a dated name"@en .

bhf:scobID
    rdf:type     owl:DatatypeProperty ;
    rdfs:domain  bhf:Class ;
    rdfs:range   xsd:integer ;
    rdfs:label   "scob ID"@en ;
    rdfs:comment "ID of an entity in the scob Database"@en .